{
 "cells": [
  {
   "cell_type": "markdown",
   "metadata": {},
   "source": [
    "# Classification"
   ]
  },
  {
   "cell_type": "markdown",
   "metadata": {},
   "source": [
    "## A simple algorithm for classification"
   ]
  },
  {
   "cell_type": "markdown",
   "metadata": {},
   "source": [
    "In binary classification using kernel methods, you can classify a test point $ x $ by comparing its distance to the centers of mass (centroids) of positive and negative examples. Here's a step-by-step derivation and explanation based on the kernelized distance approach:\n",
    "\n",
    "### Step-by-Step Derivation\n",
    "\n",
    "1. **Define the Center of Mass:**\n",
    "\n",
    "   Let $ S^+ $ and $ S^- $ be the sets of positive and negative training examples, respectively. The center of mass (centroid) in the feature space for positive examples $ \\phi(S^+) $ and negative examples $ \\phi(S^-) $ are:\n",
    "\n",
    "   $$\n",
    "   \\phi_S^+ = \\frac{1}{|S^+|} \\sum_{x_i \\in S^+} \\phi(x_i)\n",
    "   $$\n",
    "   $$\n",
    "   \\phi_S^- = \\frac{1}{|S^-|} \\sum_{x_i \\in S^-} \\phi(x_i)\n",
    "   $$\n",
    "\n",
    "2. **Distance from the Centroids:**\n",
    "\n",
    "   The squared distance from a test point $ x $ to the positive centroid $ \\phi_S^+ $ is:\n",
    "\n",
    "   $$\n",
    "   d^+(x) = \\|\\phi(x) - \\phi_S^+\\|^2\n",
    "   $$\n",
    "\n",
    "   Similarly, the squared distance from $ x $ to the negative centroid $ \\phi_S^- $ is:\n",
    "\n",
    "   $$\n",
    "   d^-(x) = \\|\\phi(x) - \\phi_S^-\\|^2\n",
    "   $$\n",
    "\n",
    "3. **Calculate the Distances:**\n",
    "\n",
    "   Using the properties of the kernel function and the centroids, we get:\n",
    "\n",
    "   $$\n",
    "   d^+(x) = \\|\\phi(x) - \\phi_S^+\\|^2 = \\|\\phi(x)\\|^2 + \\|\\phi_S^+\\|^2 - 2 \\langle \\phi(x), \\phi_S^+ \\rangle\n",
    "   $$\n",
    "   $$\n",
    "   d^-(x) = \\|\\phi(x) - \\phi_S^-\\|^2 = \\|\\phi(x)\\|^2 + \\|\\phi_S^-\\|^2 - 2 \\langle \\phi(x), \\phi_S^- \\rangle\n",
    "   $$\n",
    "\n",
    "   Substitute $ \\|\\phi(x)\\|^2 = \\kappa(x, x) $ and the inner products $ \\langle \\phi(x), \\phi_S^+ \\rangle $ and $ \\langle \\phi(x), \\phi_S^- \\rangle $:\n",
    "\n",
    "   $$\n",
    "   \\langle \\phi(x), \\phi_S^+ \\rangle = \\frac{1}{|S^+|} \\sum_{x_i \\in S^+} \\kappa(x, x_i)\n",
    "   $$\n",
    "   $$\n",
    "   \\langle \\phi(x), \\phi_S^- \\rangle = \\frac{1}{|S^-|} \\sum_{x_i \\in S^-} \\kappa(x, x_i)\n",
    "   $$\n",
    "\n",
    "   So:\n",
    "\n",
    "   $$\n",
    "   d^+(x) = \\kappa(x, x) + \\frac{1}{|S^+|^2} \\sum_{i=1}^{|S^+|} \\sum_{j=1}^{|S^+|} \\kappa(x_i, x_j) - \\frac{2}{|S^+|} \\sum_{i=1}^{|S^+|} \\kappa(x, x_i)\n",
    "   $$\n",
    "   $$\n",
    "   d^-(x) = \\kappa(x, x) + \\frac{1}{|S^-|^2} \\sum_{i=1}^{|S^-|} \\sum_{j=1}^{|S^-|} \\kappa(x_i, x_j) - \\frac{2}{|S^-|} \\sum_{i=1}^{|S^-|} \\kappa(x, x_i)\n",
    "   $$\n",
    "\n",
    "4. **Simplify the Classification Rule:**\n",
    "\n",
    "   To classify $ x $, compare $ d^+(x) $ and $ d^-(x) $. The classification rule is:\n",
    "\n",
    "   $$\n",
    "   h(x) = \\begin{cases} \n",
    "   +1 & \\text{if } d^-(x) > d^+(x) \\\\\n",
    "   -1 & \\text{otherwise}\n",
    "   \\end{cases}\n",
    "   $$\n",
    "\n",
    "   We can simplify this using the sign function. Express $ d^+(x) $ and $ d^-(x) $ in terms of kernel evaluations:\n",
    "\n",
    "   $$\n",
    "   d^+(x) = \\kappa(x, x) + \\frac{1}{|S^+|^2} \\sum_{i=1}^{|S^+|} \\sum_{j=1}^{|S^+|} \\kappa(x_i, x_j) - \\frac{2}{|S^+|} \\sum_{i=1}^{|S^+|} \\kappa(x, x_i)\n",
    "   $$\n",
    "   $$\n",
    "   d^-(x) = \\kappa(x, x) + \\frac{1}{|S^-|^2} \\sum_{i=1}^{|S^-|} \\sum_{j=1}^{|S^-|} \\kappa(x_i, x_j) - \\frac{2}{|S^-|} \\sum_{i=1}^{|S^-|} \\kappa(x, x_i)\n",
    "   $$\n",
    "\n",
    "   Thus:\n",
    "\n",
    "   $$\n",
    "   h(x) = \\text{sgn} \\left( \\frac{1}{|S^+|^2} \\sum_{i=1}^{|S^+|} \\sum_{j=1}^{|S^+|} \\kappa(x_i, x_j) - \\frac{1}{|S^-|^2} \\sum_{i=1}^{|S^-|} \\sum_{j=1}^{|S^-|} \\kappa(x_i, x_j) - \\frac{2}{|S^+|} \\sum_{i=1}^{|S^+|} \\kappa(x, x_i) + \\frac{2}{|S^-|} \\sum_{i=1}^{|S^-|} \\kappa(x, x_i) \\right)\n",
    "   $$\n",
    "\n",
    "5. **Final Classification Function:**\n",
    "\n",
    "   To simplify, let:\n",
    "\n",
    "   $$\n",
    "   b = \\frac{1}{2} \\left( \\frac{1}{|S^+|^2} \\sum_{i=1}^{|S^+|} \\sum_{j=1}^{|S^+|} \\kappa(x_i, x_j) - \\frac{1}{|S^-|^2} \\sum_{i=1}^{|S^-|} \\sum_{j=1}^{|S^-|} \\kappa(x_i, x_j) \\right)\n",
    "   $$\n",
    "\n",
    "   Therefore:\n",
    "\n",
    "   $$\n",
    "   h(x) = \\text{sgn} \\left( \\frac{1}{|S^+|} \\sum_{i=1}^{|S^+|} \\kappa(x, x_i) - \\frac{1}{|S^-|} \\sum_{i=1}^{|S^-|} \\kappa(x, x_i) - b \\right)\n",
    "   $$\n"
   ]
  }
 ],
 "metadata": {
  "language_info": {
   "name": "python"
  }
 },
 "nbformat": 4,
 "nbformat_minor": 2
}
